add AddDeduction and AddEquiv

MinimumLogic/ProofTheory/ExtensionTactic.v
@@ -7,9 +7,12 @@ Require Import Logic.GeneralLogic.ProofTheory.BasicSequentCalculus.
 Require Import Logic.MinimumLogic.Syntax.
 Require Import Logic.MinimumLogic.ProofTheory.TheoryOfSequentCalculus.
 Require Import Logic.MinimumLogic.ProofTheory.Minimum.
+Require Import Logic.MinimumLogic.ProofTheory.TheoryOfJudgement.
 
 Inductive P2D_reg: Type :=.
 Inductive D2P_reg: Type :=.
+Inductive P2D1_reg: Type :=.
+Inductive P2E_reg: Type :=.
 
 Ltac pose_proof_SC_instance n :=
   let a := get_nth P2D_reg n in
@@ -22,6 +25,20 @@ Ltac pose_proof_AX_instance n :=
   let a := get_nth D2P_reg n in
   match a with
   | fun x: unit => ?T => 
+    try pose_proof_instance_as T x
+  end.
+
+Ltac pose_proof_ND_instance n :=
+  let a := get_nth P2D1_reg n in
+  match a with
+  | fun x: unit => ?T =>
+    try pose_proof_instance_as T x
+  end.
+
+Ltac pose_proof_NE_instance n :=
+  let a := get_nth P2E_reg n in
+  match a with
+  | fun x: unit => ?T =>
     try pose_proof_instance_as T x
   end.
 
@@ -40,6 +57,37 @@ Ltac AddAxiomatization :=
   set (GammaP := Derivable2Provable) in SC;
   clearbody GammaP;
   rec_from_n (0%nat) pose_proof_AX_instance.
+
+Ltac AddDeduction :=
+  let ND := fresh "ND" in
+  let GammaD1 := fresh "GammaD1" in
+  pose proof Provable2Derivable1_Normal as ND;
+  set (GammaD1 := Provable2Derivable1) in ND;
+  clearbody GammaD1;
+  rec_from_n (0%nat) pose_proof_ND_instance.
+
+Ltac AddEquiv :=
+  let NEL :=fresh "NEL" in
+  let GammaL :=fresh "GammaL" in
+  pose proof Provable2Equiv_Normal as NEL;
+  set (GammaL := Provable2Equiv) in NEL;
+  rec_from_n (0%nat) pose_proof_NE_instance.
+
+(*GammaP : Provable L
+SC : NormalSequentCalculus L GammaP Gamma
+AX : FiniteWitnessedSequentCalculus L Gamma ->
+     NormalAxiomatization L GammaP Gamma
+minAX : MinimumAxiomatization L GammaP
+ipAX : IntuitionisticPropositionalLogic L GammaP
+
+AddSequentCalculus:
+GammaD : Derivable L
+AX : NormalAxiomatization L Gamma GammaD
+SC : NormalSequentCalculus L Gamma GammaD
+bSC : BasicSequentCalculus L GammaD
+fwSC : FiniteWitnessedSequentCalculus L GammaD
+minSC : MinimumSequentCalculus L GammaD
+ipSC : IntuitionisticPropositionalSequentCalculus L GammaD*)
 
 Instance reg_Axiomatization2SequentCalculus_SC:
   RegisterClass P2D_reg (fun SC: unit => @Axiomatization2SequentCalculus_SC) 0.
@@ -64,6 +112,58 @@ Qed.
 Instance reg_SequentCalculus2Axiomatization_minAX:
   RegisterClass D2P_reg (fun minAX: unit => @SequentCalculus2Axiomatization_minAX) 1.
 Qed.
+
+Instance reg_Axiomatization2Deduction_minMD:
+  RegisterClass P2D1_reg (fun minMD: unit => @Axiomatization2Deduction_minMD) 0.
+Qed.
+
+Instance reg_Axiomatization2BasicDeduction:
+  RegisterClass P2D1_reg (fun BD: unit => @Axiomatization2BasicDeduction) 1.
+Qed.
+
+Instance reg_Axiomatization2LogicEquiv_minME:
+  RegisterClass P2E_reg (fun minME: unit => @Axiomatization2LogicEquiv_minME) 0.
+Qed.
+
+Instance reg_Axiomatization2BasicLogicEquiv:
+  RegisterClass P2E_reg (fun BE: unit => @Axiomatization2BasicLogicEquiv) 1.
+Qed.
+
+Section Test_AddD.
+
+Context {L: Language}
+        {minL: MinimumLanguage L}
+        {GammaP: Provable L}
+        {GammaD: Derivable L}
+        {minAX: MinimumAxiomatization L GammaP}.
+
+Local Open Scope logic_base.
+Local Open Scope syntax.
+
+Lemma test_AddD: forall (x:expr), |-- x --> x.
+Proof.
+  AddDeduction.
+  Abort.
+
+End Test_AddD.
+
+Section Test_AddE.
+
+Context {L: Language}
+        {minL: MinimumLanguage L}
+        {GammaP: Provable L}
+        {GammaD: Derivable L}
+        {minAX: MinimumAxiomatization L GammaP}.
+
+Local Open Scope logic_base.
+Local Open Scope syntax.
+
+Lemma test_AddE: forall (x:expr), |-- x --> x.
+Proof.
+  AddEquiv.
+  Abort.
+
+End Test_AddE.
 
 Section Test_AddSC.
 
